GMLInit/Data/Option.lean
@@ -4,17 +4,11 @@ import GMLInit.Meta.Basic
 
 namespace Option
 
-@[simp] lemma none_map {α β} (f : α → β) : none.map f = none := rfl
-
-@[simp] lemma some_map {α β} (f : α → β) (a : α) : (some a).map f = some (f a) := rfl
-
-@[simp] lemma id_map {α} (a : Option α) : a.map id = a := by cases a <;> rfl
-
 def equiv {α β} (e : Equiv α β) : Equiv (Option α) (Option β) where
   fwd
   | some x => some (e.fwd x)
   | none => none
-  rev
+  rev  
   | some x => some (e.rev x)
   | none => none
   spec := by
